pulse/share/steel/examples/pulse/lib/Pulse.Lib.Stick.fst
@@ -15,58 +15,108 @@
 *)
 
 module Pulse.Lib.Stick
+open Pulse.Lib.Pervasives
 
-open Pulse.Lib.Core
-friend Pulse.Lib.Core
-open Steel.ST.Util
+let implication opens p q =
+  unit -> stt_unobservable unit opens p (fun _ -> q)
 
-[@@"__reduce__"; "__steel_reduce__"]
-let stick #is = implies_ #is
+let is_implication opens p q : prop =
+  squash (implication opens p q)
 
-(* Using this indirection as Steel tactic relies on 'star' instead of ** *)
-val __elim_stick
-  (#is: inames)
-  (hyp concl: vprop)
-: stt_ghost unit is
-    ((stick #is hyp concl) `star` hyp)
-    (fun _ -> concl)
+assume
+val indefinite_description_implication
+  (#opens: inames) (#p #q:vprop)
+  (_:squash (is_implication opens p q))
+: unit -> stt_ghost unit opens p (fun _ -> q) //implication opens p q
 
-let __elim_stick #is hyp concl =
-  fun #opened () -> elim_implies_gen #opened #is hyp concl
+let token (v:vprop) = v
 
-let elim_stick #is = __elim_stick #is
+let trade #opens (p q:vprop)
+: vprop
+= exists* (v:vprop). token v ** pure (is_implication opens (v ** p) q)
 
-(* Using this indirection as Steel tactic relies on 'star' instead of ** *)
-val __intro_stick
-  (#is : inames)
+```pulse
+ghost
+fn return (#a:Type u#2) (x:a)
+requires emp
+returns v:a
+ensures pure (v == x)
+{
+  x
+}
+```
+
+```pulse
+ghost //this should be unobservable, but we don't have a way to annotate that yet
+fn elim_trade #is (hyp concl: vprop)
+requires trade #is hyp concl ** hyp
+ensures concl
+opens is
+{
+  unfold (trade #is hyp concl);
+  with v. assert (token v);
+  unfold token;
+  let f = return (indefinite_description_implication #is #(reveal v ** hyp) #concl ());
+  f ();
+}
+```
+
+```pulse
+ghost
+fn intro_trade
+  (#[T.exact (`emp_inames)] is : inames)
   (hyp concl: vprop)
   (v: vprop)
   (f_elim: unit -> (
-    stt_ghost unit is
-    (v `star` hyp)
+    stt_unobservable unit is
+    (v ** hyp)
     (fun _ -> concl)
   ))
-: stt_ghost unit emp_inames
-    v
-    (fun _ -> (@==>) #is hyp concl)
+requires v
+ensures trade #is hyp concl
+{
+  let f = FStar.Squash.return_squash #(implication is (v ** hyp) concl) f_elim;
+  fold (token v);
+  fold (trade #is hyp concl);
+}
+```
 
-let __intro_stick #is hyp concl v f_elim =
-  fun #opened () ->
-     intro_implies_gen #opened #is hyp concl v
-               (fun _ -> f_elim () ())
+let sub_inv
+    (os1 : inames) 
+    (os2 : inames{inames_subset os1 os2})
+    (hyp concl:vprop)
+    (f:implication os1 hyp concl)
+: implication os2 hyp concl
+= fun _ -> sub_invs_stt_unobservable (f ()) ()
 
-let intro_stick #is = __intro_stick #is
+let sub_inv_squash
+    (os1 : inames) 
+    (os2 : inames{inames_subset os1 os2})
+    (hyp concl:vprop)
+    (f:squash (is_implication os1 hyp concl))
+: squash (is_implication os2 hyp concl)
+= let p : squash (implication os1 hyp concl) = FStar.Squash.join_squash f in
+  FStar.Squash.bind_squash p
+    (fun f ->
+      FStar.Squash.return_squash (sub_inv os1 os2 hyp concl f))
 
-let stick_sub_inv
+```pulse
+ghost
+fn trade_sub_inv
   (#os1 : inames)
   (#os2 : inames{inames_subset os1 os2})
   (hyp concl: vprop)
-: stt_ghost unit emp_inames
-    (stick #os1 hyp concl)
-    (fun _ -> stick #os2 hyp concl)
-=  intro_stick #os2 hyp concl (stick #os1 hyp concl) (fun () -> elim_stick #os1 hyp concl)
+requires trade #os1 hyp concl
+ensures trade #os2 hyp concl
+{
+  unfold trade #os1 hyp concl;
+  with v. assert (token v);
+  let _ = sub_inv_squash os1 os2 (reveal v ** hyp) concl ();
+  fold (trade #os2 hyp concl);
+}
+```
 
-let op_forall_Star (#a:Type) (p:a -> vprop) : vprop = forall_ #a p
-
-let elim_forall #a = admit()
-let intro_forall #a = admit()
+let stick #is = admit()
+let elim_stick #is = admit()
+let intro_stick #is = admit()
+let stick_sub_inv #os1 #os2 = admit()
